src/high/increasing_map.v
@@ -1,0 +1,73 @@
+From stdpp Require Import gmap.
+
+From self Require Export extra.
+
+(* NOTE: The definition uses [i < j] and not [i ≤ j] in order to make the
+lemma [increasing_map_singleton] provable. When we use [increasing_map] the
+relation [R] will always be reflexive, and hence this does not matter. The
+_knowledge_ that [R] is reflexive may not always be available however (since
+we may not know that [R] is in fact the encoding of some preorder, and hence
+this definition works best. *)
+Definition increasing_map (R : relation2 positive) (ss : gmap nat positive) :=
+  ∀ i j (s s' : positive),
+    i < j → (ss !! i = Some s) → (ss !! j = Some s') → R s s'.
+
+Lemma increasing_map_singleton R t s :
+  increasing_map R {[ t := s ]}.
+Proof. intros ????? ?%lookup_singleton_Some ?%lookup_singleton_Some. lia. Qed.
+
+Lemma increasing_map_empty R : increasing_map R ∅.
+Proof. intros ????? [=]. Qed.
+
+Lemma increasing_map_insert order m t_i s_i :
+  increasing_map order m →
+  (forall t (s : positive), m !! t = Some s → t < t_i → order s s_i) →
+  (forall t (s : positive), m !! t = Some s → t_i < t → order s_i s) →
+  increasing_map order (<[t_i := s_i]> m).
+Proof.
+  intros increasing before after.
+  intros t1 t2 s1 s2 lt.
+  destruct (decide (t_i = t1)) as [eq1|neq1];
+    destruct (decide (t_i = t2)) as [eq2|neq2];
+    subst; rewrite ?lookup_insert; rewrite ?lookup_insert_ne; try done.
+  - lia.
+  - intros [= ->] ?.
+    eapply after; done.
+  - intros ? [= ->].
+    eapply before; done.
+  - by apply increasing.
+Qed.
+
+Lemma increasing_map_insert_after order `{!Transitive order} m t_i s_i t_t s_t :
+  increasing_map order m →
+  m !! t_i = Some s_i →
+  order s_i s_t →
+  t_i < t_t →
+  (forall t_c (s_c : positive),
+    m !! t_c = Some s_c → t_i < t_c → order s_t s_c ∧ order s_c s_t) →
+  increasing_map order (<[t_t := s_t]> m).
+Proof.
+  intros increasing look sLe tLe par.
+  intros t1 t2 s1 s2 lt.
+  destruct (decide (t_t = t1)) as [eq1|neq1];
+    destruct (decide (t_t = t2)) as [eq2|neq2].
+    (* subst; rewrite ?lookup_insert; try (rewrite lookup_insert_ne; last done). *)
+  - lia.
+  - subst.
+    rewrite lookup_insert.
+    rewrite lookup_insert_ne; last done.
+    intros [= ->] ?.
+    eapply par; [done | lia].
+  - rewrite <- eq2 in *.
+    rewrite lookup_insert_ne; last done.
+    rewrite lookup_insert.
+    intros look2 [= ->].
+    pose proof (Nat.lt_total t_i t1) as [lt2|[?|?]].
+    * eapply par; done.
+    * simplify_eq. done.
+    * etrans; last apply sLe.
+      eapply increasing; [| apply look2 | apply look].
+      lia.
+  - do 2 (rewrite lookup_insert_ne; last done).
+    by apply increasing.
+Qed.
